core/properties/monotonicity/sampleMoore_monotonicity.v
@@ -14,30 +14,30 @@
 (* Moore models as counterexample to prove monotonicity of CoqTL *)
 
 
- Definition Moore_m1 : Model MooreMetamodel_Metamodel_Instance :=
-     (Build_Model MooreMetamodel_Metamodel_Instance
+ Definition Moore_m1 : Model Metamodel_Instance :=
+     (Build_Model Metamodel_Instance
         (
-            (Build_MooreMetamodel_Object State_K (BuildState  "S0" "1")) :: nil
+            (StateElement (BuildState  "S0" "1")) :: nil
         )
         (
             nil
         )
      ).
  
-Definition Moore_m2 : Model MooreMetamodel_Metamodel_Instance :=
-        (Build_Model MooreMetamodel_Metamodel_Instance
+Definition Moore_m2 : Model Metamodel_Instance :=
+        (Build_Model Metamodel_Instance
             (
-                (Build_MooreMetamodel_Object Transition_K (BuildTransition  "0")) :: 
-                (Build_MooreMetamodel_Object Transition_K (BuildTransition  "1")) ::
-                (Build_MooreMetamodel_Object State_K (BuildState  "S0" "1")) :: 
-                (Build_MooreMetamodel_Object State_K (BuildState  "S1" "0")) ::  
+                (TransitionElement (BuildTransition  "0")) :: 
+                (TransitionElement (BuildTransition  "1")) ::
+                (StateElement (BuildState  "S0" "1")) :: 
+                (StateElement (BuildState  "S1" "0")) ::  
                 nil
             )
             (
-                (Build_MooreMetamodel_Link TransitionSource_K (BuildTransitionSource (BuildTransition  "0") (BuildState  "S1" "0"))) ::
-		        (Build_MooreMetamodel_Link TransitionTarget_K (BuildTransitionTarget (BuildTransition  "0") (BuildState  "S0" "1"))) ::
-                (Build_MooreMetamodel_Link TransitionSource_K (BuildTransitionSource (BuildTransition  "1") (BuildState  "S0" "1"))) ::
-		        (Build_MooreMetamodel_Link TransitionTarget_K (BuildTransitionTarget (BuildTransition  "1") (BuildState  "S1" "0"))) ::
+                (TransitionSourceLink (BuildTransitionSource (BuildTransition  "0") (BuildState  "S1" "0"))) ::
+		        (TransitionTargetLink (BuildTransitionTarget (BuildTransition  "0") (BuildState  "S0" "1"))) ::
+                (TransitionSourceLink (BuildTransitionSource (BuildTransition  "1") (BuildState  "S0" "1"))) ::
+		        (TransitionTargetLink (BuildTransitionTarget (BuildTransition  "1") (BuildState  "S1" "0"))) ::
                 nil
             )
         ).
