transformations/Moore2Mealy/MealyWF.v
@@ -1,0 +1,45 @@
+
+Require Import Mealy MealySemantics. 
+Import String.
+
+Definition unique_names (m:MealyModel) := 
+  forall e1 e2,
+  List.In (Build_MealyMetamodel_Object State_K e1) m.(Model.modelElements) ->
+  List.In (Build_MealyMetamodel_Object State_K e2) m.(Model.modelElements) ->
+  e1.(name) = e2.(name) ->
+  e1 = e2.
+
+(** Two states with the same name are equals because a state only contains a name. *)
+Lemma always_unique_names :
+  forall m, unique_names m.
+  unfold unique_names.
+  intros m e1 e2 H1 H2 E.
+  destruct e1, e2.
+  simpl in E.
+  congruence.
+Qed.
+
+Lemma in_find : 
+  forall m n e,
+    unique_names m ->
+    List.In e (MealyMetamodel_allStates m) ->
+    e.(name) = n ->
+    List.find
+           (fun s : State => (n =? s.(name))%string)
+           (MealyMetamodel_allStates m) = 
+         Some e.
+Proof.
+  intros.
+  destruct e ; simpl in * ; subst.
+  match goal with [ |- ?F = _] => destruct F eqn:E ; [ | exfalso ] end.
+  + f_equal. 
+    apply List.find_some in E.
+    destruct E as (IN2 & EQ).
+    destruct s.
+    f_equal.
+    apply String.eqb_eq in EQ. subst ; reflexivity. 
+   + apply List.find_none with (x:={| name := n |}) in E ; [ | assumption ].
+     apply String.eqb_neq in E.
+     simpl in E.
+     contradiction.
+Qed.
