transformations/Moore2Mealy/MooreWF.v
@@ -1,0 +1,55 @@
+
+Require Import Moore MooreSemantics. 
+Import String.
+
+Definition unique_names (m:MooreModel) := 
+  forall e1 e2,
+  List.In (StateElement e1) m.(Model.modelElements) ->
+  List.In (StateElement e2) m.(Model.modelElements) ->
+  e1.(name) = e2.(name) ->
+  e1 = e2.
+
+
+Lemma in_find : 
+  forall m n e,
+    unique_names m ->
+    List.In e (MooreMetamodel_allStates m) ->
+    e.(name) = n ->
+    List.find
+           (fun s : State => (n =? s.(name))%string)
+           (MooreMetamodel_allStates m) = 
+         Some e.
+Proof.
+  intros.
+  match goal with [ |- ?F = _] => destruct F eqn:E ; [ | exfalso ] end.
+  + apply List.find_some in E.
+    destruct E as (IN2 & EQ).
+    f_equal.
+    apply H.
+    * unfold MooreMetamodel_allStates in IN2.
+      unfold MooreMetamodel_toStates in IN2.
+      apply ListUtils.optionList2List_In in IN2.
+      apply List.in_map_iff in IN2.
+      destruct IN2 as (a & T & IN2).
+      unfold get_E_Data in T.
+      destruct a. 
+      - PropUtils.inj T.
+        exact IN2.
+      - discriminate T.
+    * (* same as above *)
+      unfold MooreMetamodel_allStates in H0.
+      unfold MooreMetamodel_toStates in H0.
+      apply ListUtils.optionList2List_In in H0.
+      apply List.in_map_iff in H0.
+      destruct H0 as (a & T & H0).
+      unfold get_E_Data in T.
+      destruct a. 
+      - PropUtils.inj T.
+        exact H0.
+      - discriminate T.
+        * apply String.eqb_eq in EQ.
+          congruence.
+   + apply List.find_none with (x:=e) in E ; [ | assumption ].
+     apply String.eqb_neq in E.
+     congruence.
+Qed.
